HOL/panScript.sml
@@ -1,0 +1,151 @@
+(*
+ * actual pancake programs
+ *)
+
+open stringLib;
+open helperLib;
+open finite_mapTheory; (* flookup_thm *)
+
+open asmTheory; (* word_cmp_def *)
+open miscTheory; (* read_bytearray *)
+open panLangTheory; (* size_of_shape_def *)
+open panPtreeConversionTheory; (* parse_funs_to_ast *)
+open wordLangTheory; (* word_op_def *)
+open wordsTheory; (* n2w_def *)
+
+local
+  val f =
+    List.mapPartial
+       (fn s => case remove_whitespace s of "" => NONE | x => SOME x) o
+    String.tokens (fn c => c = #"\n")
+in
+  fun quote_to_strings q =
+    f (Portable.quote_to_string (fn _ => raise General.Bind) q)
+  end
+
+fun parse_pancake q =
+  let
+    val code = quote_to_strings q |> String.concatWith "\n" |> fromMLstring
+  in
+    EVAL “parse_funs_to_ast ^code”
+end
+
+(* ffi test *)
+
+val ffi_ast = rhs $ concl $ parse_pancake ‘
+fun fn() {
+  #num_clients(0, 0, 0, 0);
+  #num_clients(0, 0, 0, 0);
+}’;
+
+Definition ffi_sem_def:
+  ffi_sem (s:('a,'ffi) panSem$state) =
+  itree_evaluate (SND $ SND $ HD $ THE ^ffi_ast) s
+End
+
+Theorem ffi_sem_thm:
+  ffi_sem s = ARB
+Proof
+  rw[ffi_sem_def, itree_semantics_def, itree_evaluate_alt] >>
+  (* Seq *)
+  rw[itree_mrec_alt, h_prog_def, h_prog_rule_seq_def] >>
+  rw[Once itree_iter_thm, Once itree_bind_thm] >>
+  (* extcall *)
+  rw[itree_mrec_alt, h_prog_def, h_prog_rule_ext_call_def] >>
+  rw[eval_def, FLOOKUP_UPDATE] >>
+  rw[read_bytearray_def] >>
+  rw[Once itree_bind_thm] >>
+  rw[Once itree_iter_thm] >>
+  rw[Once itree_bind_thm] >>
+  (* inner thing *)
+  rw[Once itree_bind_thm] >>
+  rw[Once itree_bind_thm] >>
+  (* TODO massage bug! (not yet fixed, update when done) *)
+  rw[massage_def] >>
+  rw[Once itree_unfold, massage_thm] >>
+  rw[Once itree_unfold]
+QED
+
+(*/ loops work!
+   manual loop unrolling isn't too bad with equational rewrites
+ *)
+
+val loop_ast = rhs $ concl $ parse_pancake ‘
+fun fn() {
+  var x = 0;
+  while (x < 1) {
+    x = x + 1;
+  }
+}’;
+
+Definition loop_sem_def:
+  loop_sem (s:('a,'ffi) panSem$state) =
+  itree_evaluate (SND $ SND $ HD $ THE ^loop_ast) s
+End
+
+Definition h_prog_whilebody_cb_def[simp]:
+    h_prog_whilebody_cb p (SOME Break) s' = Ret (INR (NONE,s'))
+  ∧ h_prog_whilebody_cb p (SOME Continue) s' = Ret (INL (p,s'))
+  ∧ h_prog_whilebody_cb p NONE s' = Ret (INL (p,s'))
+  (* nice! this syntax is valid *)
+  ∧ h_prog_whilebody_cb p res s' = Ret (INR (res,s'))
+End
+
+Definition h_prog_while_cb_def[simp]:
+    h_prog_while_cb (p,s) NONE = Ret (INR (SOME Error,s))
+  ∧ h_prog_while_cb (p,s) (SOME (ValWord w))
+    = (if (w ≠ 0w)
+       then Vis (INL (p,s))
+                (λ(res,s'). h_prog_whilebody_cb p res s')
+       else Ret (INR (NONE,s)))
+  ∧ h_prog_while_cb (p,s) (SOME (ValLabel _)) = Ret (INR (SOME Error,s))
+  ∧ h_prog_while_cb (p,s) (SOME (Struct _)) = Ret (INR (SOME Error,s))
+End
+
+(* PR submitted *)
+Theorem h_prog_rule_while_alt:
+  h_prog_rule_while g p s =
+  (λ(p',s'). (h_prog_while_cb (p',s') (eval s' g))) ↻ (p,s)
+Proof
+  rw[h_prog_rule_while_def] >>
+  AP_THM_TAC >>
+  AP_TERM_TAC >>
+  rw[FUN_EQ_THM] >>
+  rw[DefnBase.one_line_ify NONE h_prog_while_cb_def] >>
+  rw[DefnBase.one_line_ify NONE h_prog_whilebody_cb_def] >>
+  rpt (PURE_TOP_CASE_TAC >> gvs[] >> rw[FUN_EQ_THM])
+QED
+
+Theorem cheat1:
+  0w < 1w (* supposed to be :4 word but weever *)
+Proof
+  cheat
+QED
+
+Theorem loop_thm:
+  loop_sem s = Tau (Tau (Tau (Ret NONE)))
+Proof
+  rw[loop_sem_def, itree_semantics_def, itree_evaluate_alt] >>
+  rw[itree_mrec_alt, h_prog_def, h_prog_rule_dec_alt] >>
+  rw[eval_def] >>
+  rw[Once itree_iter_thm, itree_bind_thm] >>
+  (* while *)
+  rw[Once h_prog_def, h_prog_rule_while_alt] >>
+  rw[Once itree_iter_thm] >>
+  rw[Once itree_iter_thm] >>
+  rw[eval_def, FLOOKUP_UPDATE, word_cmp_def, cheat1] >>
+  rw[itree_bind_thm] >>
+  (* assignment *)
+  rw[Once h_prog_def, h_prog_rule_assign_def] >>
+  rw[eval_def, FLOOKUP_UPDATE, cheat1,
+     word_op_def, is_valid_value_def, shape_of_def] >>
+  rw[Once itree_iter_thm, itree_bind_thm] >>
+  (* second while *)
+  rw[Once itree_iter_thm] >>
+  rw[Once itree_iter_thm] >>
+  rw[eval_def, FLOOKUP_UPDATE, word_cmp_def] >>
+  rw[revert_binding_def] >>
+  rw[Once itree_iter_thm, itree_bind_thm] >>
+  (* massage *)
+  rw[massage_thm]
+QED
